ironfleet/src/Dafny/Distributed/Impl/Raft/QRelations.i.dfy
@@ -14,97 +14,53 @@ predicate {:opaque} Q_RaftScheduler_Next(sched:RaftServerScheduler, sched':RaftS
   RaftServerSchedulerNext(sched, sched', ios)
 }
 
+//////////////////////////////////////////////////////////
+// ProcessPacket
+//////////////////////////////////////////////////////////
 predicate {:opaque} Q_RaftServer_Next_ProcessPacket(server:RaftServer, server':RaftServer, ios:seq<RaftIo>)
 {
   RaftServerNextProcessPacket(server, server', ios)
 }
 
-predicate Q_RaftServer_Next_ReadClock_Leader(server:RaftServer, server':RaftServer, clock:int, sent_packets:seq<RaftPacket>)
+predicate {:opaque} Q_RaftServer_Next_ProcessAppendEntries_GoodReply(server:RaftServer, server':RaftServer, raft_packet:RaftPacket, sent_packet:RaftPacket)
 {
-  RaftServerNextReadClock_Leader(server, server', clock, sent_packets)
+  && raft_packet.msg.RaftMessage_AppendEntries?
+  && sent_packet.msg.RaftMessage_AppendEntriesReply?
+  && |server.log| >= 1
+  && RaftServerNextProcessAppendEntries_GoodReply(server, server', raft_packet, sent_packet)
 }
 
-predicate Q_RaftServer_Next_ReadClock_NonLeader(server:RaftServer, server':RaftServer, clock:int, sent_packets:seq<RaftPacket>)
+predicate {:opaque} Q_RaftServer_Next_ProcessAppendEntries(server:RaftServer, server':RaftServer, raft_packet:RaftPacket, clock:int, sent_packets:seq<RaftPacket>)
 {
-  RaftServerNextReadClock_NonLeader(server, server', clock, sent_packets)
+  && raft_packet.msg.RaftMessage_AppendEntries?
+  && RaftServerNextProcessAppendEntries(server, server', raft_packet, clock, sent_packets)
 }
 
+//////////////////////////////////////////////////////////
+// ReadClock
+//////////////////////////////////////////////////////////
 predicate {:opaque} Q_RaftServer_Next_ReadClock(server:RaftServer, server':RaftServer, ios:seq<RaftIo>)
 {
   RaftServerNextReadClock(server, server', ios)
 }
 
+predicate {:opaque} Q_RaftServer_Next_ReadClock_Leader(server:RaftServer, server':RaftServer, clock:int, sent_packets:seq<RaftPacket>)
+{
+  RaftServerNextReadClock_Leader(server, server', clock, sent_packets)
+}
+
+predicate {:opaque} Q_RaftServer_Next_ReadClock_NonLeader(server:RaftServer, server':RaftServer, clock:int, sent_packets:seq<RaftPacket>)
+{
+  RaftServerNextReadClock_NonLeader(server, server', clock, sent_packets)
+}
+
+//////////////////////////////////////////////////////////
+// CommitAndApply
+//////////////////////////////////////////////////////////
 predicate {:opaque} Q_RaftServer_Next_CommitAndApply(server:RaftServer, server':RaftServer, ios:seq<RaftIo>)
 {
   RaftServerNextCommitAndApply(server, server', ios)
 }
-
-// predicate {:opaque} Q_RaftServer_Next_Process_AppendEntries(server:RaftServer, server':RaftServer, raft_packet:RaftPacket, clock:int, sent_packets:seq<RaftPacket>)
-// {
-//   // raft_packet.msg.RaftMessage_AppendEntries? && RaftServerNextProcessAppendEntries(server, server', raft_packet, clock, sent_packets)
-//   true
-// }
-
-// predicate Establish_Q_RaftServer_Next_ProcessPacket_preconditions(server:RaftServer, server':RaftServer, raft_packet:RaftPacket, clock:int, sent_packets:seq<RaftPacket>, ios:seq<RaftIo>)
-// {
-//   && sent_packets == ExtractSentPacketsFromIos(ios)
-//   && clock == SpontaneousClock(ios)
-//   // && raft_packet.msg.RaftMessage_AppendEntries?
-//   // && Q_RaftServer_Next_Process_AppendEntries(server, server', raft_packet, clock, sent_packets)
-//   && (
-//     || (raft_packet.msg.RaftMessage_Invalid? && (server == server' && sent_packets == []))
-//     || (raft_packet.msg.RaftMessage_AppendEntries? && Q_RaftServer_Next_Process_AppendEntries(server, server', raft_packet, clock, sent_packets))
-//     // || (raft_packet.msg.RaftMessage_RequestVote? && (server == server' && sent_packets == []))
-//     || (raft_packet.msg.RaftMessage_AppendEntriesReply? && (server == server' && sent_packets == []))
-//     || (raft_packet.msg.RaftMessage_RequestVote? && (server == server' && sent_packets == []))
-//     || (raft_packet.msg.RaftMessage_RequestVoteReply? && (server == server' && sent_packets == []))
-//     || (raft_packet.msg.RaftMessage_Request? && (server == server' && sent_packets == []))
-//     || (raft_packet.msg.RaftMessage_Reply? && (server == server' && sent_packets == []))
-//   )
-// }
-
-// lemma lemma_EstablishQLReplicaNextProcessPacket(server:RaftServer, server':RaftServer, raft_packet:RaftPacket, clock:int, sent_packets:seq<RaftPacket>, ios:seq<RaftIo>)
-//   requires |ios| >= 1
-//   requires ios[0].LIoOpReceive?
-//   requires |ios| >= 2 ==> (
-//     || (ios[1].LIoOpReadClock? && AllIosAreSends(ios[2..]))
-//     || (ios[1].LIoOpSend? && AllIosAreSends(ios[1..]))
-//   )
-//   requires sent_packets == ExtractSentPacketsFromIos(ios)
-//   requires Establish_Q_RaftServer_Next_ProcessPacket_preconditions(server, server', raft_packet, clock, sent_packets, ios)
-//   ensures Q_RaftServer_Next_ProcessPacket(server, server', ios)
-// {
-//   reveal Q_RaftServer_Next_Process_AppendEntries();
-
-//   reveal Q_RaftServer_Next_ProcessPacket();
-// }
-
-// lemma lemma_EstablishQRaftServerSchedulerNext(server:RaftServer, server':RaftServer, ios:seq<RaftIo>, sched:RaftServerScheduler, sched':RaftServerScheduler)
-//   requires 0 <= sched.nextActionIndex <= RaftServerNumActions() - 1
-//   requires sched.nextActionIndex == 0 ==> Q_RaftServer_Next_ProcessPacket(server, server', ios)
-//   requires sched.nextActionIndex == 1 ==> Q_RaftServer_Next_ReadClock(server, server', ios)
-//   requires sched.nextActionIndex == 2 ==> Q_RaftServer_Next_CommitAndApply(server, server', ios)
-//   requires sched.server == server
-//   requires sched'.server == server'
-//   requires sched'.nextActionIndex == (sched.nextActionIndex+1) % RaftServerNumActions()
-//   // TOPROVE
-//   ensures Q_RaftScheduler_Next(sched, sched', ios)
-// {
-//   reveal Q_RaftServer_Next_ProcessPacket();
-//   reveal Q_RaftServer_Next_ReadClock();
-//   reveal Q_RaftScheduler_Next();
-//   assert sched'.nextActionIndex == (sched.nextActionIndex + 1) % RaftServerNumActions();
-//   assert Q_RaftScheduler_Next(sched, sched', ios);
-// }
-
-// lemma lemma_EstablishQRaftServerNextProcessPacketFromTimeout(server:RaftServer, server':RaftServer, ios:seq<RaftIo>)
-//   requires |ios|==1
-//   requires ios[0].LIoOpTimeoutReceive?
-//   requires server==server'
-//   ensures Q_RaftServer_Next_ProcessPacket(server, server', ios)
-// {
-//   reveal Q_RaftServer_Next_ProcessPacket();
-// }
 
 predicate {:opaque} Q_RaftServerScheduler_Next(server:RaftServerScheduler, server':RaftServerScheduler, ios:seq<RaftIo>)
 {
