ironfleet/src/Dafny/Distributed/Impl/Raft/ServerImplNoReceiveClock.i.dfy
@@ -12,9 +12,6 @@ include "PacketParsing.i.dfy"
 include "QRelations.i.dfy"
 include "ServerImpl.i.dfy"
 include "ServerImplDelivery.i.dfy"
-// include "NetRSL.i.dfy"
-// DEBUG
-include "../../Protocol/Common/UpperBound.s.dfy"
 
 module Raft__ServerImplNoReceiveClock_i {
 
@@ -32,16 +29,18 @@ import opened Raft__CMessage_i
 import opened Raft__NetRaft_i
 import opened Raft__PacketParsing_i
 import opened Raft__QRelations_i
+import opened Raft__Server_i
 import opened Raft__ServerImpl_i
 import opened Raft__ServerImplDelivery_i
 import opened Raft__Types_i
 import opened Common__UpperBound_s
 
-method Server_Next_NoReceive_ReadClock(server_impl:ServerImpl)
-  returns (ok:bool, ghost net_event_log:seq<NetEvent>, ghost ios:seq<RaftIo>)
+method {:timeLimitMultiplier 4} Server_Next_NoReceive_ReadClock_Leader(server_impl:ServerImpl)
+  returns (ok:bool, ghost net_event_log:seq<NetEvent>, ghost ios:seq<RaftIo>, ghost raft_packets:seq<RaftPacket>)
   requires server_impl.nextActionIndex == 1
   requires server_impl.Valid()
-  modifies server_impl, server_impl.repr, server_impl.random_generator
+  requires server_impl.state.role == Leader
+  modifies server_impl, server_impl.repr, server_impl.state.random_generator
   ensures server_impl.repr == old(server_impl.repr)
   ensures server_impl.net_client != null
   ensures ok == NetClientOk(server_impl.net_client)
@@ -50,8 +49,12 @@ method Server_Next_NoReceive_ReadClock(server_impl:ServerImpl)
             && server_impl.Valid()
             && server_impl.Env() == old(server_impl.Env())
             && server_impl.nextActionIndex == old(server_impl.nextActionIndex)
-            // TOPROVE
+            && |ios| >= 1
+            && ios[0].LIoOpReadClock?
+            && SpontaneousIos(ios, 1)
             // && Q_RaftServer_Next_ReadClock(old(server_impl.AbstractifyToRaftServer()), server_impl.AbstractifyToRaftServer(), ios)
+            && raft_packets == ExtractSentPacketsFromIos(ios)
+            && Q_RaftServer_Next_ReadClock_Leader(old(server_impl.AbstractifyToRaftServer()), server_impl.AbstractifyToRaftServer(), ios[0].t as int, raft_packets)
             && OnlySentMarshallableData(net_event_log)
             && RawIoConsistentWithSpecIO(net_event_log, ios)
             && old(server_impl.Env().net.history()) + net_event_log == server_impl.Env().net.history()
@@ -76,84 +79,179 @@ method Server_Next_NoReceive_ReadClock(server_impl:ServerImpl)
   ios := ios_head;
   ok := true;
 
-  if (server_impl.role.Leader?) {
-    if (clock.t >= server_impl.next_heartbeat_time) {
-      var const_params := server_impl.config.global_config.params;
-      // Create heartbeat packets
-      var outbound_packets:seq<CPacket> := [];
-      outbound_packets := Server_CreateAppendEntriesForAll(server_impl, true);
-      assert |outbound_packets| <= |server_impl.config.global_config.server_eps| <= 0xFFFF_FFFF_FFFF_FFFF;
-      assert (forall p :: p in outbound_packets ==> CPacketIsSendable(p));
-      ok, log_tail, ios_tail := DeliverOutboundPackets(server_impl, PacketSequence(outbound_packets));
-      if (!ok) { return; }
-      ios := ios_head + ios_tail;
-      net_event_log := log_head + log_tail;
-      // print "I broadcast heartbeat!\n";
-      assert forall i::0<=i<|log_tail| ==> AbstractifyNetEventToRaftIo(log_tail[i]) == ios_tail[i];
-      assert forall i::0<=i<|log_tail| ==> log_tail[i].LIoOpSend? && ios_tail[i].LIoOpSend?;
-      assert forall i :: 1 <= i < |net_event_log| ==> net_event_log[i].LIoOpSend?;
-      assert forall i :: 0 <= i < |net_event_log| - 1 ==> net_event_log[i].LIoOpReceive? || net_event_log[i+1].LIoOpSend?;
+  if (clock.t >= server_impl.state.next_heartbeat_time) {
+    var const_params := server_impl.state.config.global_config.params;
+    // Update fields of server_impl after delivering packets
+    var next_heartbeat_time := UpperBoundedAdditionImpl(clock.t, const_params.heartbeat_timeout, const_params.max_integer_value);
+    server_impl.state := server_impl.state.(next_heartbeat_time := next_heartbeat_time);
+    // Create heartbeat packets
+    var outbound_packets:seq<CPacket> := [];
+    outbound_packets := Server_CreateAppendEntriesForAll(server_impl, true);
+    assert |outbound_packets| <= |server_impl.state.config.global_config.server_eps| <= 0xFFFF_FFFF_FFFF_FFFF;
+    assert (forall p :: p in outbound_packets ==> CPacketIsSendable(p));
+    ok, log_tail, ios_tail := DeliverOutboundPackets(server_impl, PacketSequence(outbound_packets));
+    if (!ok) { return; }
+    ios := ios_head + ios_tail;
+    net_event_log := log_head + log_tail;
+    // print "I broadcast heartbeat!\n";
+    assert forall i::0<=i<|log_tail| ==> AbstractifyNetEventToRaftIo(log_tail[i]) == ios_tail[i];
+    assert forall i::0<=i<|log_tail| ==> log_tail[i].LIoOpSend? && ios_tail[i].LIoOpSend?;
+    assert forall i :: 1 <= i < |net_event_log| ==> net_event_log[i].LIoOpSend?;
+    assert forall i :: 0 <= i < |net_event_log| - 1 ==> net_event_log[i].LIoOpReceive? || net_event_log[i+1].LIoOpSend?;
 
-      // Update fields of server_impl after delivering packets
-      var next_heartbeat_time := UpperBoundedAdditionImpl(clock.t, const_params.heartbeat_timeout, const_params.max_integer_value);
-      server_impl.next_heartbeat_time := next_heartbeat_time;
-      var raft_server := old(server_impl.AbstractifyToRaftServer());
-      var raft_server' := server_impl.AbstractifyToRaftServer();
-      assert Q_RaftServer_Next_ReadClock_Leader(raft_server, raft_server', clock.t as int, AbstractifyOutboundCPacketsToSeqOfRaftPackets(PacketSequence(outbound_packets)));
-    } else {
-      net_event_log := log_head;
-      ios := ios_head;
-    }
+    var raft_server := old(server_impl.AbstractifyToRaftServer());
+    var raft_server' := server_impl.AbstractifyToRaftServer();
+    reveal Q_RaftServer_Next_ReadClock_Leader();
+    assert Q_RaftServer_Next_ReadClock_Leader(raft_server, raft_server', clock.t as int, AbstractifyOutboundCPacketsToSeqOfRaftPackets(PacketSequence(outbound_packets)));
+    raft_packets := ExtractSentPacketsFromIos(ios);
   } else {
-    if (clock.t >= server_impl.next_election_time) {
-      var const_params := server_impl.config.global_config.params;
-      var next_election_delta := server_impl.random_generator.NextInt(
-        const_params.min_election_timeout,
-        const_params.max_election_timeout
-      );
-      print "My election timeout!!\n";
-      ios := [clock_io];
-      net_event_log := [clock_event];
-      // TODO: need to increase my term
-      if server_impl.current_term > 0xFFFF_FFFF_FFFF_FFFF - 1 {
-        ok := true;
-        return;
-      }
-      server_impl.current_term := server_impl.current_term + 1;
-      server_impl.BecomeCandidate();
-      var outbound_packets;
-      ok, outbound_packets := Server_CreateRequestVoteForAll(server_impl);
-      if (!ok) {
-        ok := true;
-        return;
-      }
-      assert |outbound_packets| <= |server_impl.config.global_config.server_eps| <= 0xFFFF_FFFF_FFFF_FFFF;
-      assert (forall p :: p in outbound_packets ==> CPacketIsSendable(p));
+    net_event_log := log_head;
+    ios := ios_head;
+    raft_packets := [];
+    assert |ios| == 1;
+    assert ios[0].LIoOpReadClock?;
+    reveal ExtractSentPacketsFromIos();
+    assert ExtractSentPacketsFromIos(ios) == [];
+    reveal Q_RaftServer_Next_ReadClock_Leader();
+  }
+}
 
-      var server_impl_before_deliver := server_impl;
-      ok, log_tail, ios_tail := DeliverOutboundPackets(server_impl, PacketSequence(outbound_packets));
-      if (!ok) { return; }
-      ios := ios_head + ios_tail;
-      net_event_log := log_head + log_tail;
-      assert net_event_log[0].LIoOpReadClock?;
-      assert forall i::0<=i<|log_tail| ==> AbstractifyNetEventToRaftIo(log_tail[i]) == ios_tail[i];
-      assert forall i::0<=i<|log_tail| ==> log_tail[i].LIoOpSend? && ios_tail[i].LIoOpSend?;
-      assert forall i :: 1 <= i < |net_event_log| ==> net_event_log[i].LIoOpSend?;
-      assert forall i :: 0 <= i < |net_event_log| - 1 ==> net_event_log[i].LIoOpReceive? || net_event_log[i+1].LIoOpSend?;
+method {:timeLimitMultiplier 4} Server_Next_NoReceive_ReadClock_NonLeader(server_impl:ServerImpl)
+  returns (ok:bool, ghost net_event_log:seq<NetEvent>, ghost ios:seq<RaftIo>, ghost raft_packets:seq<RaftPacket>)
+  requires server_impl.nextActionIndex == 1
+  requires server_impl.Valid()
+  requires server_impl.state.role != Leader
+  modifies server_impl, server_impl.repr, server_impl.state.random_generator
+  ensures server_impl.repr == old(server_impl.repr)
+  ensures server_impl.net_client != null
+  ensures ok == NetClientOk(server_impl.net_client)
+  ensures server_impl.Env() == old(server_impl.Env())
+  ensures ok ==>
+            && server_impl.Valid()
+            && server_impl.Env() == old(server_impl.Env())
+            && server_impl.nextActionIndex == old(server_impl.nextActionIndex)
+            // && Q_RaftServer_Next_ReadClock(old(server_impl.AbstractifyToRaftServer()), server_impl.AbstractifyToRaftServer(), ios)
+            && |ios| >= 1
+            && ios[0].LIoOpReadClock?
+            && SpontaneousIos(ios, 1)
+            && raft_packets == ExtractSentPacketsFromIos(ios)
+            && Q_RaftServer_Next_ReadClock_NonLeader(old(server_impl.AbstractifyToRaftServer()), server_impl.AbstractifyToRaftServer(), ios[0].t as int, raft_packets)
+            && OnlySentMarshallableData(net_event_log)
+            && RawIoConsistentWithSpecIO(net_event_log, ios)
+            && old(server_impl.Env().net.history()) + net_event_log == server_impl.Env().net.history()
+            // TODO: can I remove?
+            && forall i :: 0 <= i < |net_event_log| - 1 ==> net_event_log[i].LIoOpReceive? || net_event_log[i+1].LIoOpSend?
+{
+  ok := true;
+  net_event_log := [];
+  ios := [];
 
-      server_impl := server_impl_before_deliver;
+  var clock,clock_event := ReadClock(server_impl.net_client);
+  ghost var clock_io := LIoOpReadClock(clock.t as int);
+  ghost var ios_head := [clock_io];
+  ghost var log_head := [clock_event];
+  ghost var log_tail := [];
+  ghost var ios_tail := [];
+  net_event_log := log_head;
+  ios := ios_head;
+  ghost var preDeliveryHistory := server_impl.Env().net.history();
+  // Default return
+  net_event_log := log_head;
+  ios := ios_head;
+  ok := true;
 
-      // Update fields of server_impl after delivering packets
-      var next_election_time := UpperBoundedAdditionImpl(clock.t, next_election_delta, const_params.max_integer_value);
-      server_impl.next_election_time := next_election_time;
+  if (clock.t >= server_impl.state.next_election_time) {
+    print "My election timeout!!\n";
+    var const_params := server_impl.state.config.global_config.params;
+    var next_election_delta := server_impl.state.random_generator.NextInt(
+      const_params.min_election_timeout,
+      const_params.max_election_timeout
+    );
+    var next_election_time := UpperBoundedAdditionImpl(clock.t, next_election_delta, const_params.max_integer_value);
+    
+    server_impl.state := server_impl.state.(next_election_time := next_election_time);
 
-      var raft_server := old(server_impl.AbstractifyToRaftServer());
-      var raft_server' := server_impl.AbstractifyToRaftServer();
-      // assert RaftServerNextReadClock_NonLeader(raft_server, raft_server', clock.t as int, AbstractifyOutboundCPacketsToSeqOfRaftPackets(PacketSequence(outbound_packets)));
-    } else {
-      net_event_log := log_head;
-      ios := ios_head;
+    ios := [clock_io];
+    net_event_log := [clock_event];
+    if server_impl.state.current_term >= 0xFFFF_FFFF_FFFF_FFFF {
+      // TODO: Just report this error and continue.
+      print "[ERROR] current_term overflow!\n";
     }
+    var next_term := UpperBoundedAdditionImpl(server_impl.state.current_term, 1, 0xFFFF_FFFF_FFFF_FFFF);
+    server_impl.state := server_impl.state.(current_term := next_term);
+    server_impl.BecomeCandidate();
+    var outbound_packets;
+    outbound_packets := Server_CreateRequestVoteForAll(server_impl);
+    assert |outbound_packets| <= |server_impl.state.config.global_config.server_eps| <= 0xFFFF_FFFF_FFFF_FFFF;
+    assert (forall p :: p in outbound_packets ==> CPacketIsSendable(p));
+
+    ok, log_tail, ios_tail := DeliverOutboundPackets(server_impl, PacketSequence(outbound_packets));
+    if (!ok) { return; }
+    ios := ios_head + ios_tail;
+    net_event_log := log_head + log_tail;
+    assert net_event_log[0].LIoOpReadClock?;
+    assert forall i::0<=i<|log_tail| ==> AbstractifyNetEventToRaftIo(log_tail[i]) == ios_tail[i];
+    assert forall i::0<=i<|log_tail| ==> log_tail[i].LIoOpSend? && ios_tail[i].LIoOpSend?;
+    assert forall i :: 1 <= i < |net_event_log| ==> net_event_log[i].LIoOpSend?;
+    assert forall i :: 0 <= i < |net_event_log| - 1 ==> net_event_log[i].LIoOpReceive? || net_event_log[i+1].LIoOpSend?;
+    
+    var raft_server := old(server_impl.AbstractifyToRaftServer());
+    var raft_server' := server_impl.AbstractifyToRaftServer();
+
+    reveal Q_RaftServer_Next_ReadClock_NonLeader();
+    assert Q_RaftServer_Next_ReadClock_NonLeader(raft_server, raft_server', clock.t as int, AbstractifyOutboundCPacketsToSeqOfRaftPackets(PacketSequence(outbound_packets)));
+    raft_packets := ExtractSentPacketsFromIos(ios);
+  } else {
+    net_event_log := log_head;
+    ios := ios_head;
+    raft_packets := [];
+    assert |ios| == 1;
+    assert ios[0].LIoOpReadClock?;
+    reveal ExtractSentPacketsFromIos();
+    assert ExtractSentPacketsFromIos(ios) == [];
+    reveal Q_RaftServer_Next_ReadClock_NonLeader();
+
+  }
+}
+
+
+method Server_Next_NoReceive_ReadClock(server_impl:ServerImpl)
+  returns (ok:bool, ghost net_event_log:seq<NetEvent>, ghost ios:seq<RaftIo>)
+  requires server_impl.nextActionIndex == 1
+  requires server_impl.Valid()
+  modifies server_impl, server_impl.repr, server_impl.state.random_generator
+  ensures server_impl.repr == old(server_impl.repr)
+  ensures server_impl.net_client != null
+  ensures ok == NetClientOk(server_impl.net_client)
+  ensures server_impl.Env() == old(server_impl.Env())
+  ensures ok ==>
+            && server_impl.Valid()
+            && server_impl.Env() == old(server_impl.Env())
+            && server_impl.nextActionIndex == old(server_impl.nextActionIndex)
+            && Q_RaftServer_Next_ReadClock(old(server_impl.AbstractifyToRaftServer()), server_impl.AbstractifyToRaftServer(), ios)
+            && OnlySentMarshallableData(net_event_log)
+            && RawIoConsistentWithSpecIO(net_event_log, ios)
+            && old(server_impl.Env().net.history()) + net_event_log == server_impl.Env().net.history()
+            && forall i :: 0 <= i < |net_event_log| - 1 ==> net_event_log[i].LIoOpReceive? || net_event_log[i+1].LIoOpSend?
+{
+  ghost var raft_packets;
+  if (server_impl.state.role.Leader?) {
+    ok, net_event_log, ios, raft_packets := Server_Next_NoReceive_ReadClock_Leader(server_impl);
+    if (!ok) { return; }
+    reveal Q_RaftServer_Next_ReadClock_Leader();
+    assert Q_RaftServer_Next_ReadClock_Leader(old(server_impl.AbstractifyToRaftServer()), server_impl.AbstractifyToRaftServer(), ios[0].t as int, raft_packets);
+    reveal Q_RaftServer_Next_ReadClock();
+    assert Q_RaftServer_Next_ReadClock(old(server_impl.AbstractifyToRaftServer()), server_impl.AbstractifyToRaftServer(), ios);
+  } else {
+    ok := true;
+    net_event_log := [];
+    ios := [];
+    ok, net_event_log, ios, raft_packets := Server_Next_NoReceive_ReadClock_NonLeader(server_impl);
+    if (!ok) { return; }
+    reveal Q_RaftServer_Next_ReadClock_NonLeader();
+    assert Q_RaftServer_Next_ReadClock_NonLeader(old(server_impl.AbstractifyToRaftServer()), server_impl.AbstractifyToRaftServer(), ios[0].t as int, raft_packets);
+    reveal Q_RaftServer_Next_ReadClock();
+    assert Q_RaftServer_Next_ReadClock(old(server_impl.AbstractifyToRaftServer()), server_impl.AbstractifyToRaftServer(), ios);
   }
 }
 
