ironfleet/src/Dafny/Distributed/Impl/Raft/ServerImplProcessPacketX.i.dfy
@@ -14,7 +14,7 @@ include "PacketParsing.i.dfy"
 include "QRelations.i.dfy"
 include "ServerImpl.i.dfy"
 include "ServerImplDelivery.i.dfy"
-// include "NetRSL.i.dfy"
+include "ServerImplProcessPacketX1.i.dfy"
 
 module Raft__ServerImplProcessPacketX_i {
 
@@ -37,6 +37,7 @@ import opened Raft__QRelations_i
 import opened Raft__ServerImpl_i
 import opened Raft__Types_i
 import opened Raft__ServerImplDelivery_i
+import opened Raft__ServerImplProcessPacketX1_i
 
 //////////////////////////////////////////////////////////
 // Process request from client
@@ -50,7 +51,7 @@ method Server_Next_ProcessRequest(server_impl:ServerImpl, ghost old_net_history:
   requires server_impl.Valid()
   requires server_impl.Env().net.history() == old_net_history + [receive_event]
   requires CPacketIsSendable(rr.cpacket)
-  requires ConfigStateIsValid(server_impl.config.global_config)
+  requires ConfigStateIsValid(server_impl.state.config.global_config)
   modifies server_impl, server_impl.repr, server_impl.net_client;
   ensures server_impl.repr == old(server_impl.repr)
   ensures server_impl.net_client != null
@@ -73,15 +74,15 @@ method Server_Next_ProcessRequest(server_impl:ServerImpl, ghost old_net_history:
   var recved_msg := rr.cpacket.msg;
   ghost var ios_head := [receive_io];
   ghost var log_head := [receive_event];
-  ghost var log_tail := [];                                                                                                                                                                                                                                                                                                                                                                                                                                                                                                                                                                                                                                                                                                                                                                                                                                                                                                      
+  ghost var log_tail := [];
   ghost var ios_tail := [];
   net_event_log := log_head;
   ios := ios_head;
   ok := true;
   
-  if server_impl.role == Leader {
-    var leader_ep := server_impl.config.server_ep;
-    var leader_id := GetEndPointIndex(server_impl.config.global_config, leader_ep);
+  if server_impl.state.role == Leader {
+    var leader_id := server_impl.state.config.server_id;
+    var leader_ep := server_impl.GetMyEp();
     // create entry
     var entry;
     print "trying to create log\n";
@@ -93,22 +94,22 @@ method Server_Next_ProcessRequest(server_impl:ServerImpl, ghost old_net_history:
     }
     // Append entry to leader's log
     if (
-      1 > ServerMaxLogSize() - |server_impl.log| 
-      || !(server_impl.LastLogEntryIndex() + 1 == entry.index == |server_impl.log| as uint64)
+      1 > ServerMaxLogSize() - |server_impl.state.log| 
+      || !(server_impl.LastLogEntryIndex() + 1 == entry.index == |server_impl.state.log| as uint64)
     ) {
-      print "append failed!!!",server_impl.LastLogEntryIndex() + 1, ",", entry.index, ",", |server_impl.log| as uint64, "\n";
+      print "append failed!!!",server_impl.LastLogEntryIndex() + 1, ",", entry.index, ",", |server_impl.state.log| as uint64, "\n";
       ok := true;
       return;
     }
     server_impl.AddLogEntries([entry]);
-    server_impl.next_index := server_impl.next_index[leader_ep := entry.index + 1];
-    server_impl.match_index := server_impl.match_index[leader_ep := entry.index];
-    assert server_impl.role.Leader?;
+    server_impl.state := server_impl.state.(next_index := server_impl.state.next_index[leader_ep := entry.index + 1]);
+    server_impl.state := server_impl.state.(match_index := server_impl.state.match_index[leader_ep := entry.index]);
+    assert server_impl.state.role.Leader?;
     print "append success!!!\n";
     // Create packets
     var outbound_packets:seq<CPacket> := [];
     outbound_packets := Server_CreateAppendEntriesForAll(server_impl, false);
-    assert |outbound_packets| <= |server_impl.config.global_config.server_eps| <= 0xFFFF_FFFF_FFFF_FFFF;
+    assert |outbound_packets| <= |server_impl.state.config.global_config.server_eps| <= 0xFFFF_FFFF_FFFF_FFFF;
     assert (forall p :: p in outbound_packets ==> CPacketIsSendable(p));
     ok, log_tail, ios_tail := DeliverOutboundPackets(server_impl, PacketSequence(outbound_packets));
     if (!ok) { return; }
@@ -121,13 +122,13 @@ method Server_Next_ProcessRequest(server_impl:ServerImpl, ghost old_net_history:
     assert forall i :: 0 <= i < |net_event_log| - 1 ==> net_event_log[i].LIoOpReceive? || net_event_log[i+1].LIoOpSend?;
   } else {
     var leader_id;
-    if (server_impl.current_leader.Some?) {
-      leader_id := server_impl.current_leader.v;
+    if (server_impl.state.current_leader.Some?) {
+      leader_id := server_impl.state.current_leader.v;
     } else {
-      leader_id := GetEndPointIndex(server_impl.config.global_config, server_impl.config.server_ep);
+      leader_id := GetEndPointIndex(server_impl.state.config.global_config, server_impl.GetMyEp());
     }
     var msg := CMessage_Reply(recved_msg.seqno_req, 0, leader_id, []);
-    var packet := CPacket(rr.cpacket.src, server_impl.config.server_ep , msg);
+    var packet := CPacket(rr.cpacket.src, server_impl.GetMyEp() , msg);
     var outbound_packets := OutboundPacket(Some(packet));
     ok, log_tail, ios_tail := DeliverOutboundPackets(server_impl, outbound_packets);
     if (!ok) { return; }
@@ -145,12 +146,12 @@ method Server_Next_ProcessRequest(server_impl:ServerImpl, ghost old_net_history:
 // Process AppendEntries
 //////////////////////////////////////////////////////////
 method Server_ResetNextElectionTime(server_impl:ServerImpl) returns (ghost clock_event:NetEvent, ghost clock_io:RaftIo)
-  requires server_impl.role == Follower || server_impl.role == Candidate
+  requires server_impl.state.role == Follower || server_impl.state.role == Candidate
   requires server_impl.Valid()
   // requires history_after_recv == server_impl.Env().net.history()
-  modifies server_impl, NetClientRepr(server_impl.net_client), server_impl.random_generator
+  modifies server_impl, NetClientRepr(server_impl.net_client), server_impl.state.random_generator
   ensures clock_event.LIoOpReadClock? && clock_io.LIoOpReadClock?
-  ensures server_impl.role == old(server_impl.role)
+  ensures server_impl.state.role == old(server_impl.state.role)
   ensures server_impl.Valid()
   // ensures io and event consistent
   ensures AbstractifyNetEventToRaftIo(clock_event) == clock_io
@@ -161,193 +162,18 @@ method Server_ResetNextElectionTime(server_impl:ServerImpl) returns (ghost clock
   ensures server_impl.Env() == old(server_impl.Env())
   ensures server_impl.nextActionIndex == old(server_impl.nextActionIndex)
   ensures RawIoConsistentWithSpecIO([clock_event], [clock_io])
-  ensures server_impl.log == old(server_impl.log)
+  ensures server_impl.state.log == old(server_impl.state.log)
 {
-  var const_params := server_impl.config.global_config.params;
+  var const_params := server_impl.state.config.global_config.params;
   var clock;
   clock, clock_event := ReadClock(server_impl.net_client);
-  var next_election_delta := server_impl.random_generator.NextInt(
+  var next_election_delta := server_impl.state.random_generator.NextInt(
     const_params.min_election_timeout,
     const_params.max_election_timeout
   );
   var next_election_time := UpperBoundedAdditionImpl(clock.t, next_election_delta, const_params.max_integer_value);
-  server_impl.next_election_time := next_election_time;
+  server_impl.state := server_impl.state.(next_election_time := next_election_time);
   clock_io := LIoOpReadClock(clock.t as int);
-}
-
-method Server_HandleAppendEntries_TryToAppendAndSend(server_impl:ServerImpl, ghost old_net_history:seq<NetEvent>, rr:ReceiveResult) 
-  returns (ok:bool, ghost net_event_log:seq<NetEvent>, ghost ios:seq<RaftIo>)
-  // About recved things
-  requires rr.RRPacket?
-  requires rr.cpacket.msg.CMessage_AppendEntries?
-  // About server
-  requires server_impl.role == Follower
-  requires server_impl.Valid()
-  requires server_impl.Env().net.history() == old_net_history
-  requires CPacketIsSendable(rr.cpacket)
-  requires ConfigStateIsValid(server_impl.config.global_config)
-  modifies server_impl, server_impl.repr, server_impl.net_client
-  ensures server_impl.repr == old(server_impl.repr)
-  ensures server_impl.net_client != null
-  ensures server_impl.Env().Valid() && server_impl.Env().ok.ok() ==> ok
-  ensures server_impl.Env() == old(server_impl.Env());
-  ensures ok ==> 
-            && server_impl.Valid()
-            && server_impl.nextActionIndex == old(server_impl.nextActionIndex)
-            && AllIosAreSends(ios)
-            // TOPROVE
-            // && (|| Q_RaftServer_Next_ProcessPacket(old(server_impl.AbstractifyToRaftServer()), server_impl.AbstractifyToRaftServer(), ios)
-            //     || (&& IosReflectIgnoringUnsendable(net_event_log)
-            //        && old(server_impl.AbstractifyToRaftServer()) == server_impl.AbstractifyToRaftServer()))
-            && RawIoConsistentWithSpecIO(net_event_log, ios)
-            && OnlySentMarshallableData(net_event_log)
-            && old_net_history + net_event_log == server_impl.Env().net.history()
-            && forall i :: 0 <= i < |net_event_log| - 1 ==> net_event_log[i].LIoOpReceive? || net_event_log[i+1].LIoOpSend?
-{
-  var msg := rr.cpacket.msg;
-  var my_last_log := server_impl.GetLastLogEntry();
-  var success := 0;
-  var match_index := 0;
-  net_event_log := [];
-
-  ios := [];
-  // check whether we can put the entries
-  if msg.prev_log_index > 0xFFFF_FFFF_FFFF_FFFE 
-    && (msg.prev_log_index as int + 1 + |msg.entries| > ServerMaxLogSize())
-  {
-    ok := true;
-    print "[Error] msg.prev_log_index too large";
-    return;
-  }
-  // if |server_impl.log| > 1 {
-  //   var my_last2_log := server_impl.log[|server_impl.log| - 2];
-  //   print "msg.prev_log_index=", msg.prev_log_index, ",msg.prev_log_term=", msg.prev_log_term, ", my_last_log=(index=", my_last_log.index, ",term=", my_last_log.term, "), my_last2_log=(index=", my_last2_log.index, ",term=", my_last2_log.term, ")\n";
-  // } else{
-  //   print "msg.prev_log_index=", msg.prev_log_index, ",msg.prev_log_term=", msg.prev_log_term, ", my_last_log=(index=", my_last_log.index, ",term=", my_last_log.term, ")\n";
-  // }
-
-  var my_log_at_prev_log_index := None;
-  if (msg.prev_log_index <= my_last_log.index) {
-    my_log_at_prev_log_index := server_impl.GetLogEntry(msg.prev_log_index);
-    // TOPROVE: my_log_at_prev_log_index is not None
-  }
-  if (msg.prev_log_index == 0 
-    || (msg.prev_log_index <= my_last_log.index && my_log_at_prev_log_index.Some? && msg.prev_log_term == my_log_at_prev_log_index.v.term)
-  ) {
-    success := 1;
-    assert |msg.entries| > 0 ==> server_impl.log[msg.prev_log_index].index as int + 1 == msg.entries[0].index as int;
-    if |msg.entries| == 0 {
-      match_index := msg.prev_log_index;
-    } else {
-      server_impl.log := server_impl.log[..msg.prev_log_index+1] + msg.entries;
-      match_index := msg.entries[|msg.entries|-1].index;
-    }
-    if (msg.leader_commit > server_impl.commit_index) {
-      server_impl.commit_index := msg.leader_commit;
-    }
-    print "After appending, |log|=", |server_impl.log|, "\n";
-  } else {
-    print "Not yet uptodate, cannot append\n";
-  }
-  var send_msg := CMessage_AppendEntriesReply(server_impl.current_term, success, match_index);
-  var send_packet := CPacket(rr.cpacket.src, server_impl.config.server_ep, send_msg);
-  ghost var log_tail, ios_tail;
-  ok, log_tail, ios_tail := DeliverOutboundPackets(server_impl, OutboundPacket(Some(send_packet)));
-  if (!ok) { return; }
-  net_event_log := net_event_log + log_tail;
-  ios := ios + ios_tail;
-  assert forall i::0<=i<|log_tail| ==> AbstractifyNetEventToRaftIo(log_tail[i]) == ios_tail[i];
-  assert forall i::0<=i<|log_tail| ==> log_tail[i].LIoOpSend? && ios_tail[i].LIoOpSend?;
-  assert forall i :: 0 <= i < |net_event_log| - 1 ==> net_event_log[i].LIoOpReceive? || net_event_log[i+1].LIoOpSend?;
-}
-
-method Server_HandleAppendEntries(server_impl:ServerImpl, rr:ReceiveResult, ghost old_net_history:seq<NetEvent>, ghost receive_event:NetEvent, ghost receive_io:RaftIo) 
-  returns (ok:bool, ghost net_event_log:seq<NetEvent>, ghost ios:seq<RaftIo>)
-  // About recved things
-  requires receive_event.LIoOpReceive?
-  requires rr.RRPacket?
-  requires NetPacketIsAbstractable(receive_event.r)
-  requires rr.cpacket.msg.CMessage_AppendEntries?
-  // requires server_impl.ReceivedPacketProperties(rr.cpacket, receive_event, receive_io)
-  // About server
-  requires server_impl.Valid()
-  requires server_impl.Env().net.history() == old_net_history + [receive_event]
-  requires CPacketIsSendable(rr.cpacket)
-  requires ConfigStateIsValid(server_impl.config.global_config)
-  modifies server_impl, server_impl.repr, server_impl.net_client, server_impl.random_generator
-  ensures server_impl.repr == old(server_impl.repr)
-  ensures server_impl.net_client != null
-  ensures server_impl.Env().Valid() && server_impl.Env().ok.ok() ==> ok
-  ensures server_impl.Env() == old(server_impl.Env());
-  ensures ok ==> 
-            && server_impl.Valid()
-            && server_impl.nextActionIndex == old(server_impl.nextActionIndex)
-            // TOPROVE
-            // && (
-            //   || Q_RaftServer_Next_ProcessPacket(old(server_impl.AbstractifyToRaftServer()), server_impl.AbstractifyToRaftServer(), ios)
-            //   || rr.cpacket.src !in server_impl.config.global_config.server_eps
-            //   || (|ios| == 1 && ios[0].LIoOpReceive?)
-            // )
-            && RawIoConsistentWithSpecIO(net_event_log, ios)
-            && OnlySentMarshallableData(net_event_log)
-            && old_net_history + net_event_log == server_impl.Env().net.history()
-            && forall i :: 0 <= i < |net_event_log| - 1 ==> net_event_log[i].LIoOpReceive? || net_event_log[i+1].LIoOpSend?
-{
-  ghost var receive_io := LIoOpReceive(AbstractifyNetPacketToRaftPacket(receive_event.r));
-  var msg := rr.cpacket.msg;
-  net_event_log := [receive_event];
-  ios := [receive_io];
-
-  var success := 0;
-  var match_index := 0;
-  if (server_impl.current_term < msg.term) {
-    server_impl.current_term := msg.term;
-    server_impl.voted_for := None;
-    server_impl.role := Follower;
-  }
-  var my_last_log := server_impl.GetLastLogEntry();
-  assert server_impl.Valid();
-  // update my leader
-  if (server_impl.current_term == msg.term) {
-    if rr.cpacket.src !in server_impl.config.global_config.server_eps {
-      print "[Error] src not in server_eps\n";
-      ok := true;
-      return;
-    }
-    var src_id := GetEndPointIndex(server_impl.config.global_config, rr.cpacket.src);
-    server_impl.current_leader := Some(src_id);
-  }
-  if (server_impl.current_term == msg.term) {
-    print "Trying to append #of entries=", |msg.entries|, "\n";
-    // Reset role to follower;
-    server_impl.role := Follower;
-    // And reset Election Timeout
-    ghost var clock_event, clock_io := Server_ResetNextElectionTime(server_impl);
-    assert my_last_log.index as int == |server_impl.log| - 1;
-    assert server_impl.Valid();
-    net_event_log := net_event_log + [clock_event];
-    ios := ios + [clock_io];
-    assert net_event_log[0].LIoOpReceive?;
-    assert net_event_log[1].LIoOpReadClock?;
-    ghost var net_event_log_2:seq<NetEvent> := [];
-    ghost var ios_2:seq<RaftIo> := [];
-    var old_net_history_2 := server_impl.Env().net.history();
-    ok, net_event_log_2, ios_2 := Server_HandleAppendEntries_TryToAppendAndSend(server_impl, old_net_history_2, rr);
-    if (!ok) { return; }
-    net_event_log := net_event_log + net_event_log_2;
-    ios := ios + ios_2;
-    assert forall i::0<=i<|net_event_log_2| ==> AbstractifyNetEventToRaftIo(net_event_log_2[i]) == ios_2[i];
-    assert forall i::0<=i<|net_event_log_2| ==> net_event_log_2[i].LIoOpSend? && ios_2[i].LIoOpSend?;
-    assert forall i :: 0 <= i < |net_event_log| - 1 ==> net_event_log[i].LIoOpReceive? || net_event_log[i+1].LIoOpSend?;
-    var raft_server := old(server_impl.AbstractifyToRaftServer());
-    var raft_server' := server_impl.AbstractifyToRaftServer();
-    var raft_packet := AbstractifyCPacketToRaftPacket(rr.cpacket);
-    assert raft_packet.msg.RaftMessage_AppendEntries?;
-  } else {
-    net_event_log := [receive_event];
-    ios := [receive_io];
-    ok := true;
-  }
 }
 
 //////////////////////////////////////////////////////////
@@ -361,11 +187,11 @@ method Server_HandleAppendEntriesReply(server_impl:ServerImpl, ghost old_net_his
   requires NetPacketIsAbstractable(receive_event.r)
   requires rr.cpacket.msg.CMessage_AppendEntriesReply?
   // About server
-  requires server_impl.role == Leader
+  requires server_impl.state.role == Leader
   requires server_impl.Valid()
   requires server_impl.Env().net.history() == old_net_history + [receive_event]
   requires CPacketIsSendable(rr.cpacket)
-  requires ConfigStateIsValid(server_impl.config.global_config)
+  requires ConfigStateIsValid(server_impl.state.config.global_config)
   modifies server_impl, server_impl.repr, server_impl.net_client;
   ensures server_impl.repr == old(server_impl.repr)
   ensures server_impl.net_client != null
@@ -381,7 +207,7 @@ method Server_HandleAppendEntriesReply(server_impl:ServerImpl, ghost old_net_his
             && RawIoConsistentWithSpecIO(net_event_log, ios)
             && OnlySentMarshallableData(net_event_log)
             && old_net_history + net_event_log == server_impl.Env().net.history()
-            && forall i :: 0 <= i < |net_event_log| - 1 ==> net_event_log[i].LIoOpReceive? || net_event_log[i+1].LIoOpSend?
+            && (forall i :: 0 <= i < |net_event_log| - 1 ==> net_event_log[i].LIoOpReceive? || net_event_log[i+1].LIoOpSend?)
 {
   ghost var receive_io := LIoOpReceive(AbstractifyNetPacketToRaftPacket(receive_event.r));
   var msg := rr.cpacket.msg;
@@ -391,51 +217,53 @@ method Server_HandleAppendEntriesReply(server_impl:ServerImpl, ghost old_net_his
   ok := true;
 
   // Check and update term
-  if (server_impl.current_term < msg.term) {
-    server_impl.current_term := msg.term;
-    server_impl.voted_for := None;
-    server_impl.role := Follower;
+  if (server_impl.state.current_term < msg.term) {
+    server_impl.state := server_impl.state.(
+      current_term := msg.term, voted_for := None, role := Follower
+    );
     return;
   }
   
   var ep := rr.cpacket.src;
-  if (ep !in server_impl.config.global_config.server_eps) {
+  if (ep !in server_impl.state.config.global_config.server_eps) {
     print "[Error] src of the packet not in cluster\n";
     return;
   }
 
-  if (server_impl.role == Leader && server_impl.current_term == msg.term) {
+  if (server_impl.state.role == Leader && server_impl.state.current_term == msg.term) {
     if (msg.success == 1) {
       if (msg.match_index > MaxLogEntryIndex() as uint64 - 1) {
         print "[Error] match_index too large\n";
         return;
       }
-      if (msg.match_index + 1 > |server_impl.log| as uint64) {
+      if (msg.match_index + 1 > |server_impl.state.log| as uint64) {
         print "[Error] should not be\n";
         return;
       }
-      if (msg.match_index > server_impl.match_index[ep]) {
-        server_impl.match_index := server_impl.match_index[ep := msg.match_index];
+      if (msg.match_index > server_impl.state.match_index[ep]) {
+        server_impl.state := server_impl.state.(match_index := server_impl.state.match_index[ep := msg.match_index]);
       }
-      server_impl.next_index := server_impl.next_index[ep := server_impl.match_index[ep] + 1];
+      server_impl.state := server_impl.state.(next_index := server_impl.state.next_index[ep := server_impl.state.match_index[ep] + 1]);
       // Update commit_index
-      ok := server_impl.TryToIncreaseCommitIndexUntil(server_impl.match_index[ep]);
+      ok := server_impl.TryToIncreaseCommitIndexUntil(server_impl.state.match_index[ep]);
       if (!ok) { 
-        print "[Error] TryToIncreaseCommitIndexUntil failed, ", server_impl.commit_index, "\n";
+        print "[Error] TryToIncreaseCommitIndexUntil failed, ", server_impl.state.commit_index, "\n";
         ok := true;
         return;
       } else {
-        print "[Info] Committed up to ", server_impl.commit_index, "\n";
+        print "[Info] Committed up to ", server_impl.state.commit_index, "\n";
       }
     } else {
       var decreased_index;
-      if server_impl.next_index[ep] > LogEntrySeqSizeLimit() as uint64 {
-        decreased_index := server_impl.next_index[ep] - LogEntrySeqSizeLimit() as uint64;
+      if server_impl.state.next_index[ep] > LogEntrySeqSizeLimit() as uint64 {
+        decreased_index := server_impl.state.next_index[ep] - LogEntrySeqSizeLimit() as uint64;
       } else {
         decreased_index := 1;
       }
-      server_impl.match_index := server_impl.match_index[ep := 0];
-      server_impl.next_index := server_impl.next_index[ep := decreased_index];
+      server_impl.state := server_impl.state.(
+        match_index := server_impl.state.match_index[ep := 0], 
+        next_index := server_impl.state.next_index[ep := decreased_index]
+      );
     }
   }
 
@@ -444,7 +272,7 @@ method Server_HandleAppendEntriesReply(server_impl:ServerImpl, ghost old_net_his
 //////////////////////////////////////////////////////////
 // Process RequestVote
 //////////////////////////////////////////////////////////
-method Server_HandleReqeustVote(server_impl:ServerImpl, ghost old_net_history:seq<NetEvent>, rr:ReceiveResult, ghost receive_event:NetEvent) 
+method {:timeLimitMultiplier 2} Server_HandleReqeustVote(server_impl:ServerImpl, ghost old_net_history:seq<NetEvent>, rr:ReceiveResult, ghost receive_event:NetEvent) 
   returns (ok:bool, ghost net_event_log:seq<NetEvent>, ghost ios:seq<RaftIo>)
   // About recved things
   requires receive_event.LIoOpReceive?
@@ -455,8 +283,8 @@ method Server_HandleReqeustVote(server_impl:ServerImpl, ghost old_net_history:se
   requires server_impl.Valid()
   requires server_impl.Env().net.history() == old_net_history + [receive_event]
   requires CPacketIsSendable(rr.cpacket)
-  requires ConfigStateIsValid(server_impl.config.global_config)
-  modifies server_impl, server_impl.repr, server_impl.net_client, server_impl.random_generator
+  requires ConfigStateIsValid(server_impl.state.config.global_config)
+  modifies server_impl, server_impl.repr, server_impl.net_client, server_impl.state.random_generator
   ensures server_impl.repr == old(server_impl.repr)
   ensures server_impl.net_client != null
   ensures server_impl.Env().Valid() && server_impl.Env().ok.ok() ==> ok
@@ -481,47 +309,45 @@ method Server_HandleReqeustVote(server_impl:ServerImpl, ghost old_net_history:se
   ok := true;
 
   var granted := 0;
-  if (server_impl.current_term < msg.term) {
-    server_impl.current_term := msg.term;
-    server_impl.voted_for := None;
-    server_impl.role := Follower;
+  if (server_impl.state.current_term < msg.term) {
+    server_impl.state := server_impl.state.(current_term := msg.term, voted_for := None, role := Follower);
   }
 
-  if (server_impl.role == Leader || server_impl.role == Candidate) {
+  if (server_impl.state.role == Leader || server_impl.state.role == Candidate) {
     return;
   }
 
   var my_last_log := server_impl.GetLastLogEntry();
   if (
-    server_impl.current_term == msg.term
-    && (server_impl.voted_for == None || server_impl.voted_for == Some(msg.candidate_id))
+    server_impl.state.current_term == msg.term
+    && (server_impl.state.voted_for == None || server_impl.state.voted_for == Some(msg.candidate_id))
     && (msg.last_log_term > my_last_log.term || (msg.last_log_term == my_last_log.term && msg.last_log_index >= my_last_log.index))
   ){
     granted := 1;
     // reset election timeout before we do any change to server (to avoid proof)
     ghost var clock_event, clock_io := Server_ResetNextElectionTime(server_impl);
-    assert my_last_log.index as int == |server_impl.log| - 1;
+    assert my_last_log.index as int == |server_impl.state.log| - 1;
     assert server_impl.Valid();
     net_event_log := [receive_event, clock_event];
     ios := [receive_io, clock_io];
     assert net_event_log[0].LIoOpReceive?;
     assert net_event_log[1].LIoOpReadClock?;
     // update voted_for
-    if (msg.candidate_id >= |server_impl.config.global_config.server_eps| as uint64) {
-      if |server_impl.config.global_config.server_eps| == 3 {
-        print server_impl.config.global_config.server_eps[0], "\n";
-        print server_impl.config.global_config.server_eps[1], "\n";
-        print server_impl.config.global_config.server_eps[2], "\n";
+    if (msg.candidate_id >= |server_impl.state.config.global_config.server_eps| as uint64) {
+      if |server_impl.state.config.global_config.server_eps| == 3 {
+        print server_impl.state.config.global_config.server_eps[0], "\n";
+        print server_impl.state.config.global_config.server_eps[1], "\n";
+        print server_impl.state.config.global_config.server_eps[2], "\n";
       }
       print "[Error] candidate_id(", msg.candidate_id, ") not in cluster\n";
       return;
     }
-    server_impl.voted_for := Some(msg.candidate_id);
-    server_impl.current_leader := Some(msg.candidate_id);
+    server_impl.state := server_impl.state.(voted_for := Some(msg.candidate_id));
+    server_impl.state := server_impl.state.(current_leader := Some(msg.candidate_id));
   }
   // send reply
-  var reply_msg := CMessage_RequestVoteReply(server_impl.current_term, granted);
-  var reply_packet := CPacket(rr.cpacket.src, server_impl.config.server_ep, reply_msg);
+  var reply_msg := CMessage_RequestVoteReply(server_impl.state.current_term, granted);
+  var reply_packet := CPacket(rr.cpacket.src, server_impl.GetMyEp(), reply_msg);
   ghost var log_tail, ios_tail;
   ok, log_tail, ios_tail := DeliverOutboundPackets(server_impl, OutboundPacket(Some(reply_packet)));
   if (!ok) { return; }
@@ -546,7 +372,7 @@ method Server_HandleReqeustVoteReply(server_impl:ServerImpl, ghost old_net_histo
   requires server_impl.Valid()
   requires server_impl.Env().net.history() == old_net_history + [receive_event]
   requires CPacketIsSendable(rr.cpacket)
-  requires ConfigStateIsValid(server_impl.config.global_config)
+  requires ConfigStateIsValid(server_impl.state.config.global_config)
   modifies server_impl, server_impl.repr, server_impl.net_client
   ensures server_impl.repr == old(server_impl.repr)
   ensures server_impl.net_client != null
@@ -573,15 +399,13 @@ method Server_HandleReqeustVoteReply(server_impl:ServerImpl, ghost old_net_histo
   ios := [receive_io];
   ok := true;
 
-  if (server_impl.current_term < msg.term) {
-    server_impl.current_term := msg.term;
-    server_impl.voted_for := None;
-    server_impl.role := Follower;
+  if (server_impl.state.current_term < msg.term) {
+    server_impl.state := server_impl.state.(current_term := msg.term, voted_for := None, role := Follower);
   }
 
-  if (server_impl.role == Candidate && server_impl.current_term == msg.term) {
+  if (server_impl.state.role == Candidate && server_impl.state.current_term == msg.term) {
     // Record the vote
-    server_impl.vote_granted := server_impl.vote_granted[rr.cpacket.src := msg.vote_granted];
+    server_impl.state := server_impl.state.(vote_granted := server_impl.state.vote_granted[rr.cpacket.src := msg.vote_granted]);
     // Check for step up
     var passed:bool := server_impl.VoteRequestPassed();
     print "passed=", passed, "\n";
@@ -591,7 +415,7 @@ method Server_HandleReqeustVoteReply(server_impl:ServerImpl, ghost old_net_histo
       // Create packets
       var outbound_packets:seq<CPacket> := [];
       outbound_packets := Server_CreateAppendEntriesForAll(server_impl, true);
-      assert |outbound_packets| <= |server_impl.config.global_config.server_eps| <= 0xFFFF_FFFF_FFFF_FFFF;
+      assert |outbound_packets| <= |server_impl.state.config.global_config.server_eps| <= 0xFFFF_FFFF_FFFF_FFFF;
       assert (forall p :: p in outbound_packets ==> CPacketIsSendable(p));
       ok, log_tail, ios_tail := DeliverOutboundPackets(server_impl, PacketSequence(outbound_packets));
       if (!ok) { return; }
@@ -613,11 +437,11 @@ method Server_HandleReqeustVoteReply(server_impl:ServerImpl, ghost old_net_histo
 method Server_Next_ProcessPacketX(server_impl:ServerImpl)
   returns (ok:bool, ghost net_event_log:seq<NetEvent>, ghost ios:seq<RaftIo>)
   requires server_impl.Valid()
-  requires ConfigStateIsValid(server_impl.config.global_config)
-  modifies server_impl, server_impl.repr, server_impl.net_client, server_impl.random_generator
+  requires ConfigStateIsValid(server_impl.state.config.global_config)
+  modifies server_impl, server_impl.repr, server_impl.net_client, server_impl.state.random_generator
   ensures server_impl.repr == old(server_impl.repr)
   ensures server_impl.net_client != null
-  ensures server_impl.Env().Valid() && server_impl.Env().ok.ok() ==> ok
+  // ensures server_impl.Env().Valid() && server_impl.Env().ok.ok() ==> ok
   ensures server_impl.Env() == old(server_impl.Env())
   ensures ok ==> 
             && server_impl.Valid()
@@ -633,7 +457,7 @@ method Server_Next_ProcessPacketX(server_impl:ServerImpl)
 {
   ghost var old_net_history := server_impl.Env().net.history();
 
-  var rr, receive_event := Receive(server_impl.net_client, server_impl.config.server_ep, server_impl.config.global_config, server_impl.msg_grammar);
+  var rr, receive_event := Receive(server_impl.net_client, server_impl.GetMyEp(), server_impl.state.config.global_config, server_impl.msg_grammar);
   
   assert server_impl.Env()==old(server_impl.Env());
 
@@ -660,7 +484,7 @@ method Server_Next_ProcessPacketX(server_impl:ServerImpl)
     var msg := rr.cpacket.msg;
     if (msg.CMessage_Request? || msg.CMessage_Reply?) {
       if (msg.CMessage_Request?) {
-        print "server ", my_idx, "(", server_impl.current_term, ",is_leader=", server_impl.role.Leader?, ") received a request(", msg.seqno_req, ", ", msg.req, ")\n";
+        print "server ", my_idx, "(", server_impl.state.current_term, ",is_leader=", server_impl.state.role.Leader?, ") received a request(", msg.seqno_req, ", ", msg.req, ")\n";
         ok, net_event_log, ios := Server_Next_ProcessRequest(server_impl, old_net_history, rr, receive_event);
       } else {
         return;
@@ -668,32 +492,33 @@ method Server_Next_ProcessPacketX(server_impl:ServerImpl)
     } else {
       assert msg.CMessage_AppendEntries? || msg.CMessage_AppendEntriesReply? || msg.CMessage_RequestVote? || msg.CMessage_RequestVoteReply?;
       // ignore outside packets for inside operations
-      if (rr.cpacket.src !in server_impl.config.global_config.server_eps) {
+      if (rr.cpacket.src !in server_impl.state.config.global_config.server_eps) {
         return;
       }
-      var src_id := GetEndPointIndex(server_impl.config.global_config, rr.cpacket.src);
+      var src_id := GetEndPointIndex(server_impl.state.config.global_config, rr.cpacket.src);
       // process the message
       if (msg.CMessage_AppendEntries?) {
         // ignore packet from self
-        if (rr.cpacket.src == server_impl.config.server_ep) {
+        if (rr.cpacket.src == server_impl.GetMyEp()) {
+          ok := true;
           return;
         }
-        print "server ", my_idx, "(", server_impl.current_term, ",is_leader=", server_impl.role.Leader?, ",leader=", if server_impl.current_leader.Some? then server_impl.current_leader.v else 0xFFFF_FFFF_FFFF_FFFF, 
+        print "server ", my_idx, "(", server_impl.state.current_term, ",is_leader=", server_impl.state.role.Leader?, ",leader=", if server_impl.state.current_leader.Some? then server_impl.state.current_leader.v else 0xFFFF_FFFF_FFFF_FFFF, 
           ") received from ", src_id, "AppendEntries(|entries|=", |msg.entries|, ",prev_log_index=", msg.prev_log_index, ")\n";
         ok, net_event_log, ios := Server_HandleAppendEntries(server_impl, rr, old_net_history, receive_event, receive_io);
       } else if (msg.CMessage_AppendEntriesReply?) {
-        if (server_impl.role != Leader) {
+        if (server_impl.state.role != Leader) {
           return;
         }
-        print "server ", my_idx, "(", server_impl.current_term, ",is_leader=", server_impl.role.Leader?, ",leader=", if server_impl.current_leader.Some? then server_impl.current_leader.v else 0xFFFF_FFFF_FFFF_FFFF, 
-          ") received from ", src_id, " AppendEntriesReply(term=", msg.term, ",success=", msg.success, ",match_index=", msg.match_index, ",commit=", server_impl.commit_index, ")\n";
+        print "server ", my_idx, "(", server_impl.state.current_term, ",is_leader=", server_impl.state.role.Leader?, ",leader=", if server_impl.state.current_leader.Some? then server_impl.state.current_leader.v else 0xFFFF_FFFF_FFFF_FFFF, 
+          ") received from ", src_id, " AppendEntriesReply(term=", msg.term, ",success=", msg.success, ",match_index=", msg.match_index, ",commit=", server_impl.state.commit_index, ")\n";
         ok, net_event_log, ios := Server_HandleAppendEntriesReply(server_impl, old_net_history, rr, receive_event);
       } else if (msg.CMessage_RequestVote?) {
-        print "server ", my_idx, "(", server_impl.current_term, ",is_leader=", server_impl.role.Leader?, ",leader=", if server_impl.current_leader.Some? then server_impl.current_leader.v else 0xFFFF_FFFF_FFFF_FFFF, ",commit=", server_impl.commit_index, ") received from ", src_id, " RequestVote(term=", msg.term, ")\n";
+        print "server ", my_idx, "(", server_impl.state.current_term, ",is_leader=", server_impl.state.role.Leader?, ",leader=", if server_impl.state.current_leader.Some? then server_impl.state.current_leader.v else 0xFFFF_FFFF_FFFF_FFFF, ",commit=", server_impl.state.commit_index, ") received from ", src_id, " RequestVote(term=", msg.term, ")\n";
         ok, net_event_log, ios := Server_HandleReqeustVote(server_impl, old_net_history, rr, receive_event); 
       } else {
         assert msg.CMessage_RequestVoteReply?;
-        print "server ", my_idx, "(", server_impl.current_term, ",is_leader=", server_impl.role.Leader?, ",leader=", if server_impl.current_leader.Some? then server_impl.current_leader.v else 0xFFFF_FFFF_FFFF_FFFF, ") received from ", src_id, " RequestVoteReply(term=", msg.term, ",granted=", msg.vote_granted, ")\n";
+        print "server ", my_idx, "(", server_impl.state.current_term, ",is_leader=", server_impl.state.role.Leader?, ",leader=", if server_impl.state.current_leader.Some? then server_impl.state.current_leader.v else 0xFFFF_FFFF_FFFF_FFFF, ") received from ", src_id, " RequestVoteReply(term=", msg.term, ",granted=", msg.vote_granted, ")\n";
         ok, net_event_log, ios := Server_HandleReqeustVoteReply(server_impl, old_net_history, rr, receive_event);
         return;
       }
