ironfleet/src/Dafny/Distributed/Impl/Raft/ServerImplProcessPacketX1.i.dfy
@@ -1,0 +1,291 @@
+include "../../Common/Collections/Seqs.i.dfy"
+include "../../Common/Logic/Option.i.dfy"
+include "../../../Libraries/Math/mod_auto.i.dfy"
+include "../../Protocol/Raft/Server.i.dfy"
+include "../../Protocol/Raft/Types.i.dfy"
+include "../Common/UpperBound.i.dfy"
+include "AppInterface.i.dfy"
+include "CBroadcast.i.dfy"
+include "CMessage.i.dfy"
+include "Config.i.dfy"
+include "CTypes.i.dfy"
+include "NetRaft.i.dfy"
+include "PacketParsing.i.dfy"
+include "QRelations.i.dfy"
+include "ServerImpl.i.dfy"
+include "ServerImplDelivery.i.dfy"
+
+// DEBUG
+include "../../Protocol/Common/UpperBound.s.dfy"
+
+module Raft__ServerImplProcessPacketX1_i {
+
+import opened Native__Io_s
+import opened Native__NativeTypes_s
+import opened Collections__Seqs_i
+import opened Logic__Option_i
+import opened Math__mod_auto_i
+import opened Common__NetClient_i
+import opened Common__UpperBound_i
+import opened Environment_s
+import opened Raft__AppInterface_i
+import opened Raft__CBroadcast_i
+import opened Raft__ConfigState_i
+import opened Raft__CTypes_i
+import opened Raft__CMessage_i
+import opened Raft__NetRaft_i
+import opened Raft__PacketParsing_i
+import opened Raft__QRelations_i
+import opened Raft__Server_i
+import opened Raft__ServerImpl_i
+import opened Raft__Types_i
+import opened Raft__ServerImplDelivery_i
+import opened Common__UpperBound_s
+
+//////////////////////////////////////////////////////////
+// Process AppendEntries
+//////////////////////////////////////////////////////////
+method Server_ResetNextElectionTime(server_impl:ServerImpl) returns (ghost clock_event:NetEvent, ghost clock_io:RaftIo)
+  requires server_impl.state.role == Follower || server_impl.state.role == Candidate
+  requires server_impl.Valid()
+  // requires history_after_recv == server_impl.Env().net.history()
+  modifies server_impl, NetClientRepr(server_impl.net_client), server_impl.state.random_generator
+  ensures clock_event.LIoOpReadClock? && clock_io.LIoOpReadClock?
+  ensures server_impl.state.role == old(server_impl.state.role)
+  ensures server_impl.Valid()
+  // ensures io and event consistent
+  ensures AbstractifyNetEventToRaftIo(clock_event) == clock_io
+  // ensures history correctly changed
+  ensures old(server_impl.Env().net.history()) + [clock_event] == server_impl.Env().net.history()
+  // make sure some fields unchanged
+  ensures server_impl.repr == old(server_impl.repr)
+  ensures server_impl.Env() == old(server_impl.Env())
+  ensures server_impl.nextActionIndex == old(server_impl.nextActionIndex)
+  ensures RawIoConsistentWithSpecIO([clock_event], [clock_io])
+  ensures server_impl.state == old(server_impl.state).(next_election_time := server_impl.state.next_election_time)
+  ensures server_impl.state.next_election_time as int >= UpperBoundedAddition(clock_io.t, server_impl.state.config.global_config.params.min_election_timeout as int, UpperBoundFinite(server_impl.state.config.global_config.params.max_integer_value as int))
+  ensures server_impl.state.next_election_time as int <= UpperBoundedAddition(clock_io.t, server_impl.state.config.global_config.params.max_election_timeout as int, UpperBoundFinite(server_impl.state.config.global_config.params.max_integer_value as int))
+{
+  var const_params := server_impl.state.config.global_config.params;
+  var clock;
+  clock, clock_event := ReadClock(server_impl.net_client);
+  var next_election_delta := server_impl.state.random_generator.NextInt(
+    const_params.min_election_timeout,
+    const_params.max_election_timeout
+  );
+  var next_election_time := UpperBoundedAdditionImpl(clock.t, next_election_delta, const_params.max_integer_value);
+  server_impl.state := server_impl.state.(next_election_time := next_election_time);
+  clock_io := LIoOpReadClock(clock.t as int);
+}
+
+method {:timeLimitMultiplier 2} Server_HandleAppendEntries_TryToAppendAndSend(server_impl:ServerImpl, ghost old_net_history:seq<NetEvent>, rr:ReceiveResult, tmp_server_impl:ServerImpl) 
+  returns (ok:bool, ghost net_event_log:seq<NetEvent>, ghost ios:seq<RaftIo>)
+  // About recved things
+  requires rr.RRPacket?
+  requires rr.cpacket.msg.CMessage_AppendEntries?
+  // About server
+  requires server_impl.state.role == Follower
+  requires server_impl.Valid()
+  requires server_impl.Env().net.history() == old_net_history
+  requires CPacketIsSendable(rr.cpacket)
+  requires ConfigStateIsValid(server_impl.state.config.global_config)
+  requires tmp_server_impl == server_impl
+  modifies server_impl, server_impl.repr, server_impl.net_client
+  ensures server_impl.repr == old(server_impl.repr)
+  ensures server_impl.net_client != null
+  ensures server_impl.Env() == old(server_impl.Env());
+  ensures server_impl.state == old(server_impl.state).(log := server_impl.state.log, commit_index := server_impl.state.commit_index)
+  ensures ok ==> 
+            && server_impl.Valid()
+            && server_impl.nextActionIndex == old(server_impl.nextActionIndex)
+            && AllIosAreSends(ios)
+            && (forall i :: 0 <= i < |ios| ==> ios[i].LIoOpSend? && ios[i].s.msg.RaftMessage_AppendEntriesReply?)
+            && RawIoConsistentWithSpecIO(net_event_log, ios)
+            && OnlySentMarshallableData(net_event_log)
+            && old_net_history + net_event_log == server_impl.Env().net.history()
+            && (forall i :: 0 <= i < |net_event_log| - 1 ==> net_event_log[i].LIoOpReceive? || net_event_log[i+1].LIoOpSend?)
+            && |net_event_log| == |ios| == 1
+            && Q_RaftServer_Next_ProcessAppendEntries_GoodReply(old(server_impl.AbstractifyToRaftServer()), server_impl.AbstractifyToRaftServer(), AbstractifyCPacketToRaftPacket(rr.cpacket), ios[0].s)
+            && Q_RaftServer_Next_ProcessAppendEntries_GoodReply(tmp_server_impl.AbstractifyToRaftServer(), server_impl.AbstractifyToRaftServer(), AbstractifyCPacketToRaftPacket(rr.cpacket), ios[0].s)
+{
+  var msg := rr.cpacket.msg;
+  var my_last_log := server_impl.GetLastLogEntry();
+  var success := 0;
+  var match_index := 0;
+  net_event_log := [];
+  ios := [];
+  
+  // check whether we can put the entries
+  if msg.prev_log_index > 0xFFFF_FFFF_FFFF_FFFE 
+    && (msg.prev_log_index as int + 1 + |msg.entries| > ServerMaxLogSize())
+  {
+    ok := false;
+    print "[Error] msg.prev_log_index too large";
+    return;
+  }
+
+  var my_log_at_prev_log_index := None;
+  if (0 <= msg.prev_log_index <= my_last_log.index) {
+    my_log_at_prev_log_index := server_impl.GetLogEntry(msg.prev_log_index);
+  }
+  if (msg.prev_log_index == 0 
+    || (my_log_at_prev_log_index.Some? && msg.prev_log_term == my_log_at_prev_log_index.v.term)
+  ) {
+    success := 1;
+    assert |msg.entries| > 0 ==> server_impl.state.log[msg.prev_log_index].index as int + 1 == msg.entries[0].index as int;
+    if |msg.entries| == 0 {
+      match_index := msg.prev_log_index;
+    } else {
+      server_impl.state := server_impl.state.(log := server_impl.state.log[..msg.prev_log_index+1] + msg.entries);
+      match_index := msg.entries[|msg.entries|-1].index;
+    }
+    if (msg.leader_commit > server_impl.state.commit_index) {
+      server_impl.state := server_impl.state.(commit_index := msg.leader_commit);
+    }
+    print "After appending, |log|=", |server_impl.state.log|, "\n";
+  } else {
+    print "Not yet uptodate, cannot append\n";
+  }
+  var send_msg := CMessage_AppendEntriesReply(server_impl.state.current_term, success, match_index);
+  var send_packet := CPacket(rr.cpacket.src, server_impl.GetMyEp(), send_msg);
+  ghost var log_tail, ios_tail;
+  ok, log_tail, ios_tail := DeliverOutboundPackets(server_impl, OutboundPacket(Some(send_packet)));
+  if (!ok) { return; }
+  net_event_log := net_event_log + log_tail;
+  ios := ios + ios_tail;
+  assert forall i :: 0<=i<|log_tail| ==> AbstractifyNetEventToRaftIo(log_tail[i]) == ios_tail[i];
+  assert forall i :: 0<=i<|log_tail| ==> (
+    && log_tail[i].LIoOpSend? 
+    && ios_tail[i].LIoOpSend?
+    && ios_tail[i].s.msg.RaftMessage_AppendEntriesReply?
+  );
+  assert forall i :: 0<=i<|net_event_log|-1 ==> net_event_log[i].LIoOpReceive? || net_event_log[i+1].LIoOpSend?;
+  var raft_server := old(server_impl.AbstractifyToRaftServer());
+  var raft_server' := server_impl.AbstractifyToRaftServer();
+  var raft_recv_packet := AbstractifyCPacketToRaftPacket(rr.cpacket);
+  var raft_sent_packet := ios[0].s;
+  assert raft_recv_packet.msg.RaftMessage_AppendEntries?;
+  assert raft_sent_packet.msg.RaftMessage_AppendEntriesReply?;
+  assert |raft_server.log| >= 1;
+
+  reveal Q_RaftServer_Next_ProcessAppendEntries_GoodReply();
+  assert Q_RaftServer_Next_ProcessAppendEntries_GoodReply(raft_server, raft_server', raft_recv_packet, raft_sent_packet);
+}
+
+method {:timeLimitMultiplier 8} Server_HandleAppendEntries(server_impl:ServerImpl, rr:ReceiveResult, ghost old_net_history:seq<NetEvent>, ghost receive_event:NetEvent, ghost receive_io:RaftIo) 
+  returns (ok:bool, ghost net_event_log:seq<NetEvent>, ghost ios:seq<RaftIo>)
+  // About recved things
+  requires receive_event.LIoOpReceive?
+  requires rr.RRPacket?
+  requires NetPacketIsAbstractable(receive_event.r)
+  requires rr.cpacket.msg.CMessage_AppendEntries?
+  requires receive_io.LIoOpReceive?
+  requires receive_io.r == AbstractifyCPacketToRaftPacket(rr.cpacket)
+  requires receive_io == LIoOpReceive(AbstractifyNetPacketToRaftPacket(receive_event.r));
+  // requires server_impl.ReceivedPacketProperties(rr.cpacket, receive_event, receive_io)
+  // About server
+  requires server_impl.Valid()
+  requires server_impl.Env().net.history() == old_net_history + [receive_event]
+  requires CPacketIsSendable(rr.cpacket)
+  requires ConfigStateIsValid(server_impl.state.config.global_config)
+  modifies server_impl, server_impl.repr, server_impl.net_client, server_impl.state.random_generator
+  ensures server_impl.repr == old(server_impl.repr)
+  ensures server_impl.net_client != null
+  ensures server_impl.Env() == old(server_impl.Env());
+  ensures ok ==> 
+            && server_impl.Valid()
+            && server_impl.nextActionIndex == old(server_impl.nextActionIndex)
+            && (
+              || rr.cpacket.msg.term < server_impl.state.current_term
+              || Q_RaftServer_Next_ProcessPacket(old(server_impl.AbstractifyToRaftServer()), server_impl.AbstractifyToRaftServer(), ios)
+            )
+            && RawIoConsistentWithSpecIO(net_event_log, ios)
+            && OnlySentMarshallableData(net_event_log)
+            && old_net_history + net_event_log == server_impl.Env().net.history()
+            && (forall i :: 0 <= i < |net_event_log| - 1 ==> net_event_log[i].LIoOpReceive? || net_event_log[i+1].LIoOpSend?)
+{
+  var msg := rr.cpacket.msg;
+  net_event_log := [receive_event];
+  ios := [receive_io];
+
+  var success := 0;
+  var match_index := 0;
+  if (server_impl.state.current_term < msg.term) {
+    server_impl.state := server_impl.state.(
+      current_term := msg.term, voted_for := None, role := Follower
+    );
+  }
+  var my_last_log := server_impl.GetLastLogEntry();
+  assert server_impl.Valid();
+  // update my leader
+  if (server_impl.state.current_term == msg.term) {
+    if rr.cpacket.src !in server_impl.state.config.global_config.server_eps {
+      print "[Error] src not in server_eps\n";
+      ok := false;
+      return;
+    }
+    var src_id := GetEndPointIndex(server_impl.state.config.global_config, rr.cpacket.src);
+    server_impl.state := server_impl.state.(current_leader := Some(src_id));
+  }
+  if (server_impl.state.current_term == msg.term) {
+    print "Trying to append #of entries=", |msg.entries|, "\n";
+    // Reset role to follower;
+    server_impl.state := server_impl.state.(role := Follower);
+    // And reset Election Timeout
+    ghost var clock_event, clock_io := Server_ResetNextElectionTime(server_impl);
+    assert my_last_log.index as int == |server_impl.state.log| - 1;
+    assert server_impl.Valid();
+    assert |ios| == 1;
+    net_event_log := net_event_log + [clock_event];
+    ios := ios + [clock_io];
+    assert net_event_log[0].LIoOpReceive?;
+    assert net_event_log[1].LIoOpReadClock?;
+    assert server_impl.state.config == old(server_impl.state.config);
+    var old_net_history2 := server_impl.Env().net.history();
+    ghost var net_event_log2, ios2;
+    assert server_impl.state.log == old(server_impl.state.log);
+    assert old(server_impl.AbstractifyToRaftServer().log) == server_impl.AbstractifyToRaftServer().log;
+    var tmp_server_impl := server_impl;
+    ok, net_event_log2, ios2 := Server_HandleAppendEntries_TryToAppendAndSend(server_impl, old_net_history2, rr, tmp_server_impl);
+    if (!ok) { return; }
+    reveal Q_RaftServer_Next_ProcessAppendEntries_GoodReply();
+    assert Q_RaftServer_Next_ProcessAppendEntries_GoodReply(old(server_impl.AbstractifyToRaftServer()), server_impl.AbstractifyToRaftServer(), AbstractifyCPacketToRaftPacket(rr.cpacket), ios2[0].s);
+
+    net_event_log := net_event_log + net_event_log2;
+    ios := ios + ios2;
+    assert forall i :: 0<=i<|net_event_log2| ==> AbstractifyNetEventToRaftIo(net_event_log2[i]) == ios2[i];
+    assert forall i :: 0<=i<|net_event_log2| ==> (
+      && net_event_log2[i].LIoOpSend?
+      && ios2[i].LIoOpSend?
+      && ios2[i].s.msg.RaftMessage_AppendEntriesReply?
+    );
+    assert forall i :: 0<=i<|net_event_log|-1 ==> net_event_log[i].LIoOpReceive? || net_event_log[i+1].LIoOpSend?;
+
+    var raft_server := old(server_impl.AbstractifyToRaftServer());
+    var raft_server' := server_impl.AbstractifyToRaftServer();
+    var raft_packet := AbstractifyCPacketToRaftPacket(rr.cpacket);
+    assert raft_packet.msg.RaftMessage_AppendEntries?;
+
+    assert AbstractifyCPacketToRaftPacket(rr.cpacket) == ios[0].r;
+    assert clock_io.t == ios[1].t;
+    // assert forall io :: io in ios[2..] ==> io.LIoOpSend?;
+    lemma_OnlySentPacketsLeft(ios, 2);
+    assert ExtractSentPacketsFromIos(ios) == ExtractSentPacketsFromIos(ios[2..]) == ExtractSentPacketsFromIos(ios2);
+
+    reveal Q_RaftServer_Next_ProcessAppendEntries();
+    assert Q_RaftServer_Next_ProcessAppendEntries(raft_server, raft_server', raft_packet, clock_io.t, ExtractSentPacketsFromIos(ios));
+
+    // assert |ios| == 3;
+    // assert ios[0].LIoOpReceive?;
+    // assert ios[1].LIoOpReadClock?;
+    reveal Q_RaftServer_Next_ProcessPacket();
+    assert Q_RaftServer_Next_ProcessPacket(raft_server, raft_server', ios);
+  } else {
+    net_event_log := [receive_event];
+    ios := [receive_io];
+    ok := true;
+    // reveal Q_RaftServer_Next_ProcessPacket();
+  }
+}
+
+}
